src/Compiler.v
@@ -1,8 +1,9 @@
-Require Core. 
-Require RTL. 
+Require Core Front RTL Flat CSE FirstOrder. 
 
-Definition compile Phi t  (a : forall Var, Core.action Phi Var t) : forall Var, RTL.block Phi Var t.  
-intros. 
+
+Definition compile Phi t  (a : forall Var, Front.action Phi Var t) : forall Var, Flat.block Phi Var t.  
+intros.
+apply Flat.compile. 
 apply RTL.nblock_to_block. 
 apply RTL.compile. 
 apply a. 
@@ -12,18 +13,38 @@ Defined.
 Lemma compile_correct (Phi : Core.state) t a :
   let block := compile Phi t a in 
   forall st Delta, 
-  RTL.eval_block Phi st t (block Core.eval_type) Delta =
-     Core.Sem.eval_action (a Core.eval_type) st Delta. 
+  Flat.eval_block Phi st t (block Core.eval_type) Delta =
+     Front.Sem.eval_action (a Core.eval_type) st Delta. 
 Proof. 
   intros. 
+
   rewrite <- RTL.CPS_compile_correct.        
   rewrite <- RTL.nblock_compile_correct.
+  rewrite <- Flat.compile_correct. 
   unfold block. unfold compile. 
   reflexivity. 
 Qed. 
 
 Print Assumptions compile_correct. 
 
-                      
-        
-  
+Definition fo_compile Phi t  (a : forall Var, Front.action Phi Var t) :  FirstOrder.block Phi t.  
+intros.
+apply FirstOrder.compile. 
+apply Flat.compile. 
+apply RTL.nblock_to_block. 
+apply RTL.compile. 
+apply a. 
+Defined. 
+
+
+Definition fo_cse_compile Phi t  (a : forall Var, Front.action Phi Var t) :  FirstOrder.block Phi t.  
+intros.
+apply FirstOrder.compile. 
+apply CSE.cse_block. 
+apply Flat.compile. 
+apply RTL.nblock_to_block. 
+apply RTL.compile. 
+apply a. 
+Defined. 
+
+Print Opaque Dependencies fo_cse_compile.
