src/RTL.v
@@ -1,5 +1,6 @@
 Require Import Common. 
 Require Import Core.   
+Require Import Front. 
   
 Section t. 
   Variable Phi : state. 
@@ -11,7 +12,7 @@ Section t.
   Inductive bind (t : type) : Type := 
   | bind_expr :  expr R t ->  bind t
   | bind_reg_read : var Phi (Treg t) -> bind t
-  | bind_regfile_read : forall n, var Phi (Tregfile n t) -> R (Tlift (Tint n)) -> bind t. 
+  | bind_regfile_read : forall n, var Phi (Tregfile n t) -> R ( (Tint n)) -> bind t. 
     
   Inductive telescope (A : Type): Type :=
   | telescope_end : A -> telescope A
@@ -19,11 +20,11 @@ Section t.
     
   (* nested effects *)
   Inductive neffect  : Type :=
-  | neffect_guard : forall (guard : expr R Bool), list (neffect) -> neffect 
+  | neffect_guard : forall (guard : expr R Tbool), list (neffect) -> neffect 
   | neffect_reg_write : forall t, var Phi (Treg t) -> R t -> neffect
-  | neffect_regfile_write : forall n t, var Phi (Tregfile n t) -> R (Tlift (Tint n)) -> R t -> neffect. 
+  | neffect_regfile_write : forall n t, var Phi (Tregfile n t) -> R ( (Tint n)) -> R t -> neffect. 
 
-  Definition nblock t := telescope (R t * expr R Bool * list neffect)%type. 
+  Definition nblock t := telescope (R t * expr R Tbool * list neffect)%type. 
   
   Fixpoint compose {A B}
                    (tA : telescope  A)
@@ -36,7 +37,7 @@ Section t.
 
   Definition compose_block {t B} 
                            (tA : nblock t)
-                           (f : R t -> expr R Bool -> list neffect -> telescope B) :
+                           (f : R t -> expr R Tbool -> list neffect -> telescope B) :
     telescope B :=
     compose tA (fun x => match x with ((r,g),e) => f r g e end). 
   Hint Unfold compose_block. 
@@ -50,7 +51,7 @@ Section t.
   (** This 'smart constructor' reduces the size of the guard, by using
   the fact that [true] is a neutral element for [&&] *)
   
-  Definition andb (a b : expr R Bool): expr R Bool :=
+  Definition andb (a b : expr R Tbool): expr R Tbool :=
     match a, b with 
       | Econstant Tbool x, o 
       | o, Econstant Tbool x => if x then o else (#b false)%expr
@@ -70,9 +71,9 @@ Section t.
   Arguments map {T F F'} G l _. 
 
   (**  The compilation function itself *)  
-  Definition compile_inner (unit : R Unit) t (a : action Phi R t) : telescope (R t * expr R Bool * list neffect).  
+  Definition compile_inner (unit : R Tunit) t (a : action Phi R t) : telescope (R t * expr R Tbool * list neffect).  
   refine (
-      let f := fix compile t (a : action Phi R t) : telescope (R t * expr R Bool * list neffect):= 
+      let f := fix compile t (a : action Phi R t) : telescope (R t * expr R Tbool * list neffect):= 
           match a with 
             | Return t exp =>  
                 x <- (bind_expr _ exp); 
@@ -139,15 +140,15 @@ Section t.
 
   
   Inductive effect  : sync -> Type :=
-  | effect_reg_write : forall t,  R t -> R Bool -> effect (Treg t)
-  | effect_regfile_write : forall n t,  R t -> R (Tlift (Tint n)) -> R Bool -> 
+  | effect_reg_write : forall t,  R t -> R Tbool -> effect (Treg t)
+  | effect_regfile_write : forall n t,  R t -> R ( (Tint n)) -> R Tbool -> 
                                                 effect (Tregfile n t). 
   
   Definition effects := Tuple.of_list (option ∘ effect) Phi. 
   
   Definition init_effects : effects := Tuple.init sync (option ∘ effect) (fun t : sync => None) Phi. 
 
-  Definition block t := telescope (R t * expr R Bool *  effects). 
+  Definition block t := telescope (R t * expr R Tbool *  effects). 
     
   Notation "e :-- t1 ; t2 " := (compose t1 (fun e => t2)) (right associativity, at level 80, e1 at next level).
   Arguments Tuple.set {T F l t} _ _ _.  
@@ -155,13 +156,13 @@ Section t.
   Definition nblock_to_block {t} (B : nblock t) : block t. 
   unfold block, nblock in *. 
   
-  Definition inversion_effect_Treg t (e : effect (Treg t)) : (R t * R Bool) :=
+  Definition inversion_effect_Treg t (e : effect (Treg t)) : (R t * R Tbool) :=
     match e with 
       | effect_reg_write _ x y => (x,y)
     end. 
 
   Definition inversion_effect_Tregfile t n (e: effect (Tregfile n t)): 
-    (R t * R (Tlift (Tint n)) *R Bool) :=
+    (R t * R ( (Tint n)) *R Tbool) :=
     match e with 
       | effect_regfile_write _ _ x y z => (x,y,z)
     end. 
@@ -201,7 +202,7 @@ Section t.
   Defined. 
                                                                        
 
-  Fixpoint compile_neffect (G : expr R Bool) (E : neffect) (B : effects) : telescope effects :=
+  Fixpoint compile_neffect (G : expr R Tbool) (E : neffect) (B : effects) : telescope effects :=
     match E with               
       | neffect_guard guard L => 
                     let compile_neffects := fix compile_neffects G l U :=
@@ -221,7 +222,7 @@ Section t.
     end.  
 
     
-  Fixpoint compile_neffects (G : expr R Bool)(l : list neffect)  (T : effects) :
+  Fixpoint compile_neffects (G : expr R Tbool)(l : list neffect)  (T : effects) :
     telescope effects :=
     match l with 
       | nil =>  & T
@@ -270,11 +271,11 @@ Section t.
                 | false => Delta
             end
       | neffect_reg_write t v w =>                                               
-          Core.Diff.add Phi Delta (Treg t) v w 
+          Front.Diff.add Phi Delta (Treg t) v w 
       | neffect_regfile_write  n t v adr w  =>  
           let rf := Tuple.get Phi (Tregfile n t) v st in                          
             let rf := Regfile.set rf adr  w in 
-              Core.Diff.add Phi Delta (Tregfile n t) v rf            
+              Front.Diff.add Phi Delta (Tregfile n t) v rf            
     end. 
   
     Fixpoint eval_neffects ( l : list (neffect eval_type)) Delta : updates :=
@@ -348,30 +349,6 @@ Section t.
             end). 
     Defined. 
     apply eval_effect. 
-    (* Definition eval_effect (a : sync) :    *)
-    (*   (option ∘ effect eval_type) a -> *)
-    (*   var Phi a -> updates -> updates.  *)
-    
-    (* refine (fun  eff =>  *)
-    (*           match eff with  *)
-    (*               | Some eff =>   *)
-    (*                   match eff in effect _ s return var Phi s -> updates -> updates with    *)
-    (*                     |  effect_reg_write t val we =>   *)
-    (*                          fun v Delta => *)
-    (*                            if we then Tuple.set v (Some val) Delta else Delta *)
-    (*                     |  effect_regfile_write n t val adr we =>  *)
-    (*                          fun v Delta =>  *)
-    (*                            if we then  *)
-    (*                              let rf := Tuple.get Phi (Tregfile n t) v st in                     *)
-    (*                              let rf := Regfile.set rf adr val in  *)
-    (*                                  Tuple.set v (Some rf) Delta             *)
-    (*                            else *)
-    (*                              Delta *)
-    (*                   end *)
-    (*               | None => fun v Delta => Delta *)
-    (*           end).  *)
-    (* Defined.  *)
-
     Defined. 
 
     Fixpoint eval_block t  (T : block eval_type t) :
@@ -390,24 +367,19 @@ Section t.
   
      
   End sem. 
-
-
-  (* Notation "x <-- e1 ; e2" := (telescope_bind  _ _ _ e1 (fun x => e2)) (right associativity, at level 80, e1 at next level).   *)
-  (* Notation " & e " := (telescope_end  _ _ e) (at level 71).  *)
-  (* Notation "[< r , g , e >] :- t1 ; t2 " := (compose  _ t1 (fun r g e => t2)) (right associativity, at level 80, t1 at next level).  *)
   
   Section correctness. 
   
     
     Notation C := (compile_inner eval_type tt). 
-    Lemma eval_andb_true x y : (eval_expr Bool (andb eval_type x y)) = (eval_expr Bool x && eval_expr Bool y)%bool.
+    Lemma eval_andb_true x y : (eval_expr Tbool (andb eval_type x y)) = (eval_expr Tbool x && eval_expr Tbool y)%bool.
     Proof. 
       Require Import Equality Bool. 
       
       dependent destruction x; dependent destruction y; simpl;
       repeat match goal with 
-                 c : constant0 B |- _ => destruct c
-               | x : eval_type Bool |- _ => destruct x
+                 c : constant B |- _ => destruct c
+               | x : eval_type Tbool |- _ => destruct x
                | _ => idtac
              end; rewrite ?andb_true_r, ?andb_true_l, ?andb_false_l , ?andb_false_r ; reflexivity.  
     Qed. 
@@ -428,7 +400,7 @@ Section t.
 
     Notation "B / Delta " := (eval_nblock st _ B Delta). 
     Theorem CPS_compile_correct t (a : action Phi eval_type t)  Delta:
-      eval_nblock st _ (C t a ) Delta =  (Core.Sem.eval_action a st Delta).
+      eval_nblock st _ (C t a ) Delta =  (Front.Sem.eval_action a st Delta).
     Proof. 
       revert Delta. 
       induction a. 
@@ -445,7 +417,7 @@ Section t.
         
         induction T. destruct a as [[rA gA] eA]. 
         simpl in *. 
-        case_eq (eval_expr Bool gA); intros H.  simpl.
+        case_eq (eval_expr Tbool gA); intros H.  simpl.
         unfold compose_block; simpl compose.  
         induction (C u (f rA)). simpl. destruct a as [[rB gB] eB]. simpl. 
         * rewrite eval_neffects_append. rewrite eval_andb_true. rewrite H. simpl. reflexivity. 
@@ -486,7 +458,7 @@ Section t.
           rewrite <- convert_commute. simpl. reflexivity.
         + simpl. 
           rewrite <- convert_commute. simpl. 
-          case_eq (convert eval_type ([Tlift (Tint n); t])%list exprs). 
+          case_eq (convert eval_type ([ (Tint n); t])%list exprs). 
           intros adr [value tt] H.  simpl. simpl in tt.           
           reflexivity. 
 
@@ -518,26 +490,7 @@ Section correctness2.
   Ltac t := simpl; intuition; try match goal with
                                     | [ H : _ |- _ ] => rewrite H; auto
                                 end.
-  
-  Lemma prefold_idempotent : forall T B (F : T -> Type) (l : list T)
-                               (up : forall a, F a -> var l a -> B -> B),
-                               (forall a (x : F a) v acc, up a x v acc = acc)
-                               -> forall s f ol acc, Tuple.prefold l up s f ol acc = acc.
-  induction s; t.
-  Qed.
-    
-  Lemma prefold_2  : forall T B (F : T -> Type ) (l : list T)
-                       (up : forall a, F a -> var l a -> B -> B), 
-                       forall s f (ol : Tuple.of_list F s), 
-                         (forall a  v acc, up a (Tuple.get _ _ v ol) (f _ v) acc = acc) ->
-                         forall acc, Tuple.prefold l up s f ol acc = acc. 
-  Proof. 
-  induction s; t. destruct ol as [hd tl]. rewrite IHs.  
-  specialize (H a var_0). simpl in H. 
-  apply H.   
-  intros. specialize (H a0 (var_S v)). simpl in H. apply H. 
-  Qed. 
- 
+   
   
   Lemma eval_effect_init Phi st Delta : eval_effects Phi st (init_effects Phi eval_type) Delta = Delta. 
   Proof.
@@ -555,18 +508,17 @@ Section correctness2.
       apply functional_extensionality.
       apply H.
   Qed.
-  
      
   Lemma my_ind Phi (R : type -> Type) (P : neffect Phi R -> Prop) :
-    (forall (guard : expr R Bool) ,
+    (forall (guard : expr R Tbool) ,
        P (neffect_guard Phi  R guard [])) ->
-    (forall (guard : expr R Bool) a l ,
+    (forall (guard : expr R Tbool) a l ,
        P a -> P (neffect_guard Phi  R guard l) ->
        P (neffect_guard Phi  R guard (a :: l))) ->
     (forall (t : type) (v : var Phi (Treg t)) (r : R t),
        P (neffect_reg_write  Phi R t v r)) ->
     (forall (n : nat) (t : type) (v : var Phi (Tregfile n t))
-       (r : R (Tlift (Tint n))) (r0 : R t),
+       (r : R ( (Tint n))) (r0 : R t),
        P (neffect_regfile_write Phi R n t v r r0)) ->
     forall n : neffect Phi R, P n. 
   Proof.
@@ -592,7 +544,7 @@ Section correctness2.
   
   Lemma eval_neffect_cons Phi st guard a l Delta: 
     eval_neffect Phi st (neffect_guard Phi eval_type guard (a :: l)) Delta = 
-                 (if eval_expr Bool guard
+                 (if eval_expr Tbool guard
                   then eval_neffects Phi st l (eval_neffect Phi st a Delta)
                   else Delta).
   Proof. 
@@ -608,14 +560,14 @@ Section correctness2.
     end. 
 
   Lemma folder Phi st guard l Delta: eval_neffect Phi st (neffect_guard  Phi eval_type guard l) Delta 
-                                         = if eval_expr Bool guard then eval_neffects Phi st l Delta else Delta.
+                                         = if eval_expr Tbool guard then eval_neffects Phi st l Delta else Delta.
   Proof. 
     reflexivity. 
   Qed. 
     
 
   
-  Notation "[[ x ]]" := (eval_expr Bool x). 
+  Notation "[[ x ]]" := (eval_expr Tbool x). 
   Arguments Tuple.set {T F l t} _ _ _.
   Arguments Tuple.get {T F l t} _ _. 
 
@@ -870,315 +822,6 @@ Section correctness2.
 
     Qed. 
   
-(*
-  
-  Definition compile  t (a : action Phi R t) : telescope (R t * expr R Bool * list effect).  
-  refine (
-      let f := fix compile t (a : action Phi R t) : telescope (R t * expr R Bool * list effect):= 
-          match a with 
-            | Return t exp =>  
-                x <- (bind_expr _ exp); 
-                & (x, #b true, nil)
-            | Bind t u A F => 
-                [< rA, gA, eA >] :- compile _ A;
-                [< rB, gB, eB >] :- compile _ (F rA); 
-                & (rB, andb gA gB, List.app eA eB)             
-            | Assert exp => 
-                x <- (bind_expr _ exp); 
-                & (varunit, !x, nil)%expr
-            | Primitive args res p exprs => _
-            (* | Try A =>  *)
-            (*     [< rA, gA, eA >] :- compile _ A; *)
-            (*     let e := effect_guard gA eA in *)
-            (*       & (varunit, #b true, [e])%list *)
-            (*     (* & (varunit, gA, eA) *) *)
-            | OrElse t A A' => 
-                [< rA, gA, eA >] :- compile _ A;
-                [< rA', gA', eA' >] :- compile _ A';
-                let e := effect_guard gA eA in 
-                let e' := effect_guard ((~ gA) &&  gA')%expr eA' in 
-                  r <- (bind_expr _ (Emux _ _ gA (!rA) (!rA'))%expr); 
-                  & ( r , (gA || gA')%expr , [e;e'])%list
-          end in f t a).
-  (* primitive *)
-  revert exprs. 
-  refine (match p with
-            | register_read t v => _
-            | register_write t v => _
-            | regfile_read n t v p => _
-            | regfile_write n t v p => _
-          end); clear p; intros exprs. 
-  (* register read *)
-  refine (x <- (bind_reg_read _ v); &(x, #b true, nil)). 
-  (* register write *)
-  refine ( let env := convert _ exprs in 
-             let w := fst env in 
-               x <- bind_expr _ w; 
-           let e := ([effect_reg_write _ v x])%list  in 
-             &( varunit, #b true, e)
-         ). 
-  (* register file read *)
-  refine ( let env := convert _ exprs in 
-             let adr := fst env in 
-               adr <- bind_expr _ adr; 
-           x <- bind_regfile_read _ _ v _ adr; 
-           &( x, #b true, nil)
-         ). 
-  (* register file write *)
-  refine ( let env := convert _ exprs in 
-             match env with 
-               | (adr, (w, _)) => 
-                   adr <- bind_expr _ adr; 
-                   w <- bind_expr _ w;
-                   let e :=  ([effect_regfile_write _ _ v _ adr w])%list in                      
-                     &( varunit, #b true, e)                      
-             end
-         ). 
-    (* or else *)
-  
-  Defined. 
-  
-  Definition wrap t (T : preblock t) : block. 
-  Proof. 
-    eapply compose. apply T. 
-    intros _ g e. 
-    refine (            let e := effect_guard g e in 
-                          & (cons e nil )). 
-  Defined. 
-  End defs. 
-  
-  (** * Semantics *)
-  Section sem. 
-    Variable st : eval_state Phi. 
-    Definition eval_bind t (b : bind eval_type t) : (eval_type t).
-    refine (match b with
-              | bind_expr x =>  (eval_expr _ x)
-              | bind_reg_read v => (Tuple.get _ _ v st)
-              | bind_regfile_read n v p adr => 
-                  let rf := Tuple.get Phi (Tregfile n t) v st in
-                    Regfile.get rf (Word.unsigned adr)                
-            end
-           ). 
-    Defined. 
-    
-    Definition up {A} (x : option A) y := match x with None => y | Some y => y end.  
-                                                                
-    Fixpoint eval_effect (e :effect eval_type) (Delta : updates) : updates :=    
-      match e with 
-        | effect_guard g l' => 
-            let fix eval_effects l Delta := 
-                match l with 
-                  | nil => Delta
-                  | cons e q =>  
-                      let Delta := eval_effect e Delta in 
-                        eval_effects q Delta
-                end in     
-              match eval_expr _ g with 
-                | true =>  (* match eval_effects l' Delta with *)
-                    (*     | Some Delta => Some Delta *)
-                    (*     | None => Some Delta *)
-                        (* end                         *)
-                    eval_effects l' Delta
-                | false => Delta
-            end
-      | effect_reg_write t v w =>                                               
-          Core.Diff.add Phi Delta (Treg t) v w 
-      | effect_regfile_write  n t v p adr w  =>  
-          let rf := Tuple.get Phi (Tregfile n t) v st in                          
-            let rf := Regfile.set rf (Word.unsigned adr) w in 
-              Core.Diff.add Phi Delta (Tregfile n t) v rf            
-    end. 
-  
-    Fixpoint eval_effects ( l : list (effect eval_type)) Delta : updates :=
-      match l with 
-        | nil =>  Delta
-        | cons e q => (* do Delta <- eval_effect e Delta;  *)
-            let Delta :=  (eval_effect e Delta) in 
-            eval_effects q Delta
-      end. 
-  
-    Lemma fold_eval_effects :
-      (fix eval_effects l Delta := 
-       match l with 
-                | nil =>  Delta
-                | cons e q => 
-                    let Delta := (eval_effect e Delta) in 
-                      (* do Delta <- eval_effect e Delta;  *)
-                      eval_effects q Delta
-       end)= eval_effects .
-    Proof. 
-      unfold eval_effects. reflexivity.
-    Qed. 
-    
-    (* Lemma eval_effects_cons  t q Delta :  *)
-    (*   eval_effects (t :: q) Delta = do Delta' <- eval_effect  t Delta; eval_effects q Delta'.  *)
-    (* Proof. *)
-    (*   reflexivity.  *)
-    (* Qed.  *)
-    
-    (* Lemma eval_effect_guard (gA : expr eval_type Bool) eA Delta:  *)
-    (*   eval_expr  _ gA = true -> *)
-    (*   eval_effect  (effect_guard eval_type gA eA) Delta = eval_effects eA Delta.  *)
-    (* Proof.  *)
-    (*   intros. simpl. rewrite (fold_eval_effects).  *)
-    (*   rewrite H. reflexivity.  *)
-    (* Qed.  *)
-
-    Fixpoint eval_preblock t  (T : preblock  eval_type t) :
-      updates -> option (eval_type t * updates) := 
-      match T with
-        | telescope_bind arg bind cont => 
-            fun Delta => 
-              let res := eval_bind _ bind in
-              eval_preblock _ (cont res) Delta
-        | telescope_end (p, g, e) => fun Delta =>
-                                      let g := eval_expr _ g  in             
-                                      if g then                                         
-                                        Some (p, eval_effects e Delta)
-                                      else None
-    end. 
-  
-  
-    Fixpoint eval_block (a : block eval_type) {struct a}: updates ->  updates :=
-      match a with
-        | telescope_bind arg bind cont => 
-            fun Delta => 
-              let res  := eval_bind _ bind in 
-                eval_block (cont res) Delta
-        | telescope_end effects => eval_effects effects
-      end. 
-    
-  End sem. 
-
-
-  Notation "x <-- e1 ; e2" := (telescope_bind  _ _ _ e1 (fun x => e2)) (right associativity, at level 80, e1 at next level).  
-  Notation " & e " := (telescope_end  _ _ e) (at level 71). 
-  Notation "[< r , g , e >] :- t1 ; t2 " := (compose  _ t1 (fun r g e => t2)) (right associativity, at level 80, t1 at next level). 
-  
-  Section correctness. 
-  
-    
-    
-    Notation C := (compile eval_type tt). 
-    Lemma eval_andb_true x y : (eval_expr Bool (andb eval_type x y)) = (eval_expr Bool x && eval_expr Bool y)%bool.
-    Proof.
-      Require Import Equality. 
-      dependent destruction x. simpl. 
-    Admitted.  
-
-    Lemma eval_effects_append  st e f (Delta : updates) : 
-      eval_effects st (e ++ f) Delta = 
-                   eval_effects st f (eval_effects st e Delta).              
-    Proof. 
-      revert Delta. 
-      induction e. 
-      + reflexivity. 
-      + intros Delta.
-        
-        simpl. rewrite IHe. reflexivity.  
-
-    Qed. 
-
-    Variable st : eval_state Phi. 
-
-    Notation "B / Delta " := (eval_preblock st _ B Delta). 
-    Theorem CPS_compile_correct t (a : action Phi eval_type t)  Delta:
-      eval_preblock st _ (C t a ) Delta =  (Core.Sem.eval_action a st Delta).
-    Proof. 
-      revert Delta. 
-      induction a. 
-      - intros.  reflexivity. 
-      - intros Delta. simpl. unfold  Sem.Dyn.Bind. rewrite <- IHa.
-        transitivity (do ed <- (C t a) / Delta ; 
-                      let (e,d) := ed in 
-                      eval_preblock st u (C u (f e)) d
-                   ); 
-        [|destruct  ((C t a) / Delta) as [[ e d ]| ]; simpl; easy]. 
-        clear IHa H.
-        generalize (C t a) as T. intros T. clear a.
-        
-        induction T. destruct a as [[rA gA] eA]. 
-        simpl in *. 
-        case_eq (eval_expr Bool gA); intros H.  simpl.
-        induction (C u (f rA)). destruct a as [[rB gB] eB]. simpl. 
-        * rewrite eval_effects_append. rewrite eval_andb_true. rewrite H. simpl. reflexivity. 
-        * simpl. rewrite H0. reflexivity.         
-
-        * induction (C u (f rA)). destruct a as [[rB gB] eB]. simpl. 
-          rewrite eval_andb_true. rewrite H. reflexivity.  
-          simpl. rewrite H0. reflexivity. 
-        * simpl. rewrite H. reflexivity.
-
-      - simpl. intros. 
-          Ltac t :=
-            repeat match goal with 
-                     | |- context [check ?x ; ?y] => 
-                         let H := fresh "check" in 
-                           case_eq x; intros H
-                   end. 
-          t; trivial. 
-      -                         (* primitive *)
-      intros. destruct p.  
-        +  simpl. reflexivity. 
-        + simpl.
-              
-          set (x := DList.to_tuple eval_expr exprs). 
-          replace (x) with (fst x, snd x) by (destruct x; reflexivity).
-
-          Lemma convert_commute  l (dl : DList.T (expr eval_type) l): map  _ _ _ (eval_expr) l (convert _ l dl) = DList.to_tuple (eval_expr) dl. 
-          Proof. 
-            induction dl. simpl. reflexivity. 
-            simpl. f_equal. apply IHdl. 
-          Qed. 
-          simpl. 
-    
-          replace (eval_expr t (fst (convert eval_type [t] exprs))) with (fst x). reflexivity. 
-          subst x. rewrite <- convert_commute. simpl. reflexivity.  
-
-        + simpl. 
-          rewrite <- convert_commute. simpl. reflexivity.
-        + simpl. 
-          rewrite <- convert_commute. simpl. 
-          case_eq (convert eval_type ([Tlift (W p); t])%list exprs). 
-          intros adr [value tt] H.  simpl. simpl in tt.           
-          reflexivity. 
-
-      - intros. simpl.   unfold Sem.Dyn.OrElse. 
-        rewrite <- IHa1, <- IHa2 . clear IHa1 IHa2. 
-        generalize (C t a1); intros T; generalize (C t a2); intros T'. 
-        induction T as [[[rA gA] eA] |]; simpl.
-        induction T' as [[[rA' gA'] eA'] |]. simpl compose.
-        t. simpl. rewrite check0. simpl.  t. reflexivity. 
-        simpl. rewrite check0. simpl. t; reflexivity.  
-        simpl. rewrite H. reflexivity. 
-        simpl. rewrite H. reflexivity.
-
-    Qed.
-End correctness. 
-End t. 
-Arguments telescope_bind {Phi R A arg}  _ _.  
-Notation "'DO' X <- E ; F" := (telescope_bind E (fun X => F)).  
-Notation "'RETURN' X" := (telescope_end _ _ _ X). 
-Arguments bind_expr  {Phi R t} _%expr. 
-Notation "[: v ]" := (bind_reg_read _ _ _ v).   
-(* Section test.  *)
-(*   Require Import MOD.  *)
-(*   Definition Z (t : type) := unit.  *)
-(*   Eval compute in compile _ Z _ _  (iterate 5 Z) .  *)
-
-(*   Eval compute in compile _ Z _ _ (done 5 Z).  *)
-
-(* End test.  *)
-
-(* Section test2.  *)
-(*   Require Import Isa.  *)
-(*   Eval compute in compile _ _ 0 _ (loadi_rule 5 (fun _ => nat)).  *)
-
-(*   Eval compute in compile _ _ 0 _ (store_rule 5 (fun _ => nat)).  *)
-
-(* End test2.  *)
-
-*)
 End correctness2. 
 
 
