src/Flat.v
@@ -1,0 +1,440 @@
+Require Common Core Front RTL.
+
+Require Equality. 
+Section t. 
+  Variable Phi : Core.state. 
+  
+  Notation updates := (Common.Tuple.of_list (Common.comp option  Core.eval_sync) Phi). 
+  
+  Section defs. 
+    Import Core Common. 
+    Variable Var : type -> Type. 
+    
+    Inductive expr : type -> Type :=
+    | Eread : forall t,  var Phi (Treg t) -> expr t
+    | Eread_rf : forall n t, var Phi (Tregfile n t) -> Var (Tint n) -> expr t 
+    | Ebuiltin : forall (args : list type) (res : type),
+                   builtin args res ->
+                   DList.T Var args ->
+                   expr res
+    | Econstant : forall ty : type, constant ty -> expr ty
+    | Emux : forall t : type,
+               Var Tbool ->  Var t -> Var t -> expr  t
+    | Efst : forall (l : list type) (t : type),
+               Var (Ttuple (t :: l)) -> expr t
+    | Esnd : forall (l : list type) (t : type),
+               Var (Ttuple (t :: l)) -> expr (Ttuple l)
+    | Enth : forall (l : list type) (t : type),
+               var l t -> Var (Ttuple l) -> expr t
+    | Etuple : forall l : list type,
+                 DList.T (Var) l -> expr  (Ttuple l). 
+        
+    Inductive telescope (A : Type): Type :=
+    | telescope_end : A -> telescope A
+    | telescope_bind : forall arg, expr arg -> (Var arg -> telescope A) -> telescope A. 
+        
+    Fixpoint compose {A B}
+                     (tA : telescope  A)
+                     (f : A -> telescope  B) :
+      telescope  B :=
+      match tA with
+        | telescope_end e => f e
+        | telescope_bind arg b cont => telescope_bind _  arg b (fun x => compose (cont x) f)
+      end.
+    Notation "e :-- t1 ; t2 " := (compose t1 (fun e => t2)) (right associativity, at level 80, e1 at next level).
+      
+    Inductive effect  : sync -> Type :=
+    | effect_reg_write : forall t,  Var t -> Var Tbool -> effect (Treg t)
+    | effect_regfile_write : forall n t,  Var t -> Var (Tint n) -> Var Tbool -> 
+                                     effect (Tregfile n t). 
+    
+    Definition effects := Tuple.of_list (option ∘ effect) Phi. 
+    
+    Definition block t := telescope (Var t * Var Tbool *  effects). 
+    Notation "x :- e1 ; e2" := (telescope_bind  _ _  e1 (fun x => e2)) (right associativity, at level 80, e1 at next level).  
+    Notation " & e " := (telescope_end _  e) (at level 71). 
+    
+    
+    Definition compile_expr t (e : Front.expr Var t) : telescope (Var t).
+    refine (
+        let fix fold t (e : Front.expr Var t) :=
+            let fix of_list (l : list type) (x : DList.T (Front.expr Var) l) : telescope (DList.T Var l) :=
+                match x in  (DList.T _ l)
+                   return
+                   (telescope (DList.T Var l)) with 
+                      | DList.nil => & ([])%dlist
+                      | DList.cons t q dt dq => 
+                          x  :-- fold t dt;
+                          dq :--   of_list q dq;   
+                          &  (x :: dq)%dlist
+                end in
+              
+              match e with
+                | Front.Evar t v => & v
+                | Front.Ebuiltin args res f x => 
+                    x :-- of_list args x; 
+                    y :- Ebuiltin args res f x; 
+                    &y 
+                | Front.Econstant ty c => c :- Econstant _ c; &c
+                | Front.Emux t c l r => 
+                    c :-- fold _ c;
+                    l :-- fold _ l;
+                    r :-- fold _ r;
+                    ret :- (Emux t c l r) ;
+                    & ret
+                | Front.Efst l t x => 
+                    x :-- fold _ x; ret :- Efst l t x; & ret
+                | Front.Esnd l t x => 
+                    x :-- fold _ x; ret :- Esnd l t x; & ret
+                | Front.Enth l t m x => 
+                    x :-- fold _ x; ret :- Enth l t m x; & ret
+                | Front.Etuple l exprs => 
+                    exprs :-- of_list l exprs; ret :- Etuple l exprs; &ret
+              end in fold t e).
+    Defined. 
+    
+    Fixpoint compile_exprs l (x: DList.T (Front.expr Var) l) :  telescope (DList.T Var l) :=
+      match x in  (DList.T _ l)
+         return
+         (telescope (DList.T Var l)) with 
+        | DList.nil => & ([])%dlist
+        | DList.cons t q dt dq => 
+            x  :-- compile_expr t dt;
+            dq :--   compile_exprs q dq;   
+            &  (x :: dq)%dlist
+      end. 
+    
+    Lemma compile_exprs_fold : 
+      (fix of_list (l : list Core.type)
+           (x0 : Common.DList.T
+                       (Front.expr Var) l)
+           {struct x0} :
+       telescope 
+                   (Common.DList.T Var l) :=
+       match
+         x0 in (Common.DList.T _ l0)
+          return
+          (telescope (Common.DList.T Var l0))
+       with
+         | Common.DList.nil => & Common.DList.nil
+         | Common.DList.cons t1 q0 dt dq =>
+             x1 :-- compile_expr t1 dt;
+             dq0 :-- of_list q0 dq; & Common.DList.cons x1 dq0
+       end) = compile_exprs. 
+    Proof. reflexivity. Qed. 
+    
+    Definition compile_effects (e : RTL.effects Phi Var)  : effects. 
+    unfold effects. refine  (Tuple.map _ Phi e).
+    intros a x.
+    refine (match x with
+              | None => None
+              | Some x => match x with 
+                           | RTL.effect_reg_write t v g => 
+                               Some (effect_reg_write t v g)
+                           | RTL.effect_regfile_write n t v adr g =>
+                               Some (effect_regfile_write n t v adr g)
+                         end
+            end).
+    
+    Defined. 
+    
+    Definition compile t  (b : RTL.block Phi Var t) : block t.     
+    refine (let fold := fix fold t (b : RTL.block Phi Var t) : block t :=
+                match b with 
+                  | RTL.telescope_end x => 
+                      match x with 
+                          (r, g,e) => g :-- compile_expr _ g; & (r,g,compile_effects e)
+                        end
+                  | RTL.telescope_bind a bd k => 
+                      match bd with
+                        | RTL.bind_expr x => 
+                            x :-- compile_expr _ x ; fold _ (k x)
+                        | RTL.bind_reg_read x => 
+                            x :- Eread a x; fold _ (k x)
+                        | RTL.bind_regfile_read n x x0 => 
+                            x :- Eread_rf n a x x0; fold _ (k x)
+                      end
+                end in fold t b                         
+           ). 
+      Defined. 
+  End defs. 
+  Section sem. 
+    
+    Variable st : Core.eval_state Phi. 
+    
+    Definition eval_expr (t : Core.type) (e : expr Core.eval_type t) : Core.eval_type t. 
+    refine ( 
+        let fix eval_expr t (e : expr Core.eval_type t) {struct e} : Core.eval_type t:=
+            match e with
+              | Eread t v => (Common.Tuple.get _ _ v st)
+              | Eread_rf n t v adr =>  
+                  let rf := Common.Tuple.get Phi (Core.Tregfile n t) v st in
+                    Common.Regfile.get rf (adr)                
+
+              | Ebuiltin args res f exprs => 
+                  let exprs := 
+                      Common.DList.to_tuple  
+                            (fun (x : Core.type) (X : Core.eval_type x) => X)
+                            exprs
+                  in
+                    Core.builtin_denotation args res f exprs
+              | Emux t b x y => if b then x else y 
+              | Econstant ty c => c
+              | Etuple l exprs => 
+                  Common.DList.to_tuple (fun _ X => X) exprs
+              | Enth l t v e => 
+                  Common.Tuple.get l t v e
+              | Efst l t  e => 
+                  Common.Tuple.fst e
+              | Esnd l t  e => 
+                  Common.Tuple.snd e
+            end 
+        in eval_expr t e).  
+    Defined. 
+        
+    Definition eval_effects (e : effects Core.eval_type) (Delta : updates) : updates.  
+    unfold effects in e. 
+    
+    (* refine (Tuple.fold Phi _ e Delta).  *)
+    refine (Common.Tuple.map3 _ Phi e st Delta). 
+    Import Common Core.
+    Definition eval_effect (a : Core.sync) :   
+      (Common.comp option (effect Core.eval_type)) a ->
+      Core.eval_sync a -> (Common.comp option Core.eval_sync) a -> (Common.comp option Core.eval_sync) a. 
+    
+    refine (fun  eff => 
+              match eff with 
+                | Some eff =>  
+                    match eff in effect _ s return eval_sync s -> (option ∘ eval_sync) s -> (option ∘ eval_sync) s  with 
+                      |  effect_reg_write t val we => 
+                           fun _ old => 
+                             match old with 
+                               | Some _ => old
+                               | None => if we then Some val else None
+                             end
+                      |  effect_regfile_write n t val adr we => 
+                           fun rf old =>
+                             match old with 
+                               | Some _ => old 
+                               | None => 
+                                   if we then 
+                                     let rf := Regfile.set rf adr val in 
+                                       Some rf
+                                   else 
+                                     None                                       
+                             end
+                    end
+                | None => fun _ old => old            
+              end). 
+    Defined. 
+    apply eval_effect. 
+    Defined. 
+    
+    Fixpoint eval_telescope { A B} (F : A -> B) (T : telescope  eval_type A) :=
+      match T with 
+        | telescope_end X => F X
+        | telescope_bind arg bind cont =>
+            let res := eval_expr arg bind in 
+              eval_telescope F (cont res)
+      end. 
+    
+    Definition eval_block  t  (T : block eval_type t) Delta :
+      option (eval_type t * updates) := 
+      eval_telescope (fun x => match x with (p,g,e)  =>
+                                             if g : bool then                              
+                                               Some (p, eval_effects e Delta)
+                                             else None end) T. 
+  End sem.
+End t.  
+
+Notation "e :-- t1 ; t2 " := (compose _ _  t1 (fun e => t2)) (right associativity, at level 80, e1 at next level).
+Notation "x :- e1 ; e2" := (telescope_bind _ _ _ _ (e1) (fun x => e2)) (right associativity, at level 80, e1 at next level).  
+Notation " & e " := (telescope_end _   _ _ e) (at level 71). 
+
+
+Section correctness. 
+  Import Equality.
+  
+  Lemma compile_effects_correct Phi st   e : 
+    forall Delta, 
+      eval_effects Phi st (compile_effects Phi Core.eval_type e) Delta =
+                 RTL.eval_effects Phi st e Delta. 
+  Proof. 
+    induction Phi. simpl. auto. 
+    simpl; intros. destruct e. destruct st. destruct Delta. case_eq c; intros. 
+    dependent destruction e2. simpl. 
+    destruct c0.    f_equal. apply IHPhi. 
+    f_equal. auto. 
+    f_equal. auto. 
+    f_equal. auto. 
+  Qed. 
+  
+  Hint Resolve compile_effects_correct. 
+  
+  Lemma foo {Phi R A B C} (T: telescope Phi R A) (f : A -> telescope  Phi R B)  (g : B -> telescope Phi R C) :
+    (X :-- (Y :-- T; f Y); (g X) )= (Y :-- T; X :-- f Y; g X).
+  Proof.
+    induction T. reflexivity. simpl.
+    f_equal.
+    Require Import  FunctionalExtensionality.
+    apply functional_extensionality.
+    apply H.
+  Qed.
+  
+  
+  Section compile_expr. 
+    Context {A B : Type}. 
+    Context {E : A -> B}.  
+    Variable (Phi : Core.state) (st : Core.eval_state Phi). 
+    Notation Ev := (eval_telescope Phi st E). 
+    
+    Section compile_exprs. 
+      Notation P := (fun t e => 
+                       forall  (f : Core.eval_type t -> telescope _ _ A), 
+                         Ev(r :-- compile_expr Phi Core.eval_type t e; f r) = 
+                           Ev (f (Front.eval_expr t e))). 
+      Lemma compile_exprs_correct : forall l dl f,         
+                                      Common.DList.Forall _ _ P l dl ->                    
+                                      Ev (Y :-- compile_exprs Phi Core.eval_type l dl; f Y) =
+                                         Ev (f (Common.DList.map Front.eval_expr dl )). 
+      Proof. 
+        induction dl. simpl. reflexivity. 
+        simpl. intros. rewrite foo. destruct H. rewrite H. rewrite foo. simpl. apply IHdl. auto. 
+      Qed. 
+    End compile_exprs. 
+    Lemma compile_expr_correct t e (f : Core.eval_type t -> telescope _ _ A): 
+      Ev (r :-- compile_expr Phi Core.eval_type t e; f r) = Ev (f (Front.eval_expr t e)). 
+    Proof. 
+      revert e.
+      induction e using Front.expr_ind_alt; try reflexivity. 
+      
+      Ltac t :=
+        match goal with 
+            |- context [ (_ :-- _ :-- _; _ ; _) ] => rewrite foo
+          | H : context [ _ :-- _ ; _ ] |- _ => rewrite H ; clear H
+      end.
+      
+      { simpl. rewrite (compile_exprs_fold Phi Core.eval_type). repeat rewrite foo; simpl.
+        rewrite compile_exprs_correct; auto.  simpl.  repeat f_equal. 
+        rewrite Common.DList.map_to_tuple_commute. reflexivity. }       
+      
+      {simpl; repeat t; reflexivity.   }
+      {simpl; repeat t; reflexivity.   }
+      {simpl; repeat t; reflexivity.   }
+      {simpl; repeat t; reflexivity.   }
+      
+      { simpl. rewrite (compile_exprs_fold Phi Core.eval_type). repeat rewrite foo; simpl.
+        rewrite compile_exprs_correct; auto.  simpl.  repeat f_equal.
+        
+        rewrite Common.DList.map_to_tuple_commute. reflexivity. }       
+    
+    Qed. 
+  End compile_expr. 
+  
+  Lemma compile_correct Phi st t (b : RTL.block Phi Core.eval_type t) : 
+    forall Delta, 
+      eval_block Phi st t (compile Phi Core.eval_type t b) Delta = RTL.eval_block Phi st t b Delta. 
+  Proof. 
+    intros.
+    induction b.
+    simpl. destruct a as [[r g] e]; simpl.
+    unfold eval_block. 
+    
+    
+    rewrite (compile_expr_correct Phi st Core.Tbool g). simpl. 
+    destruct (Front.eval_expr Core.Tbool g); repeat f_equal.
+    
+    apply compile_effects_correct. 
+    
+    simpl. rewrite <- H. clear H. 
+    unfold eval_block. destruct b; try reflexivity. 
+    
+    rewrite (compile_expr_correct Phi st arg e) . reflexivity.  
+  Qed. 
+End correctness. 
+  
+
+Section equiv. 
+  Import Core. 
+  Variable U V : type -> Type. 
+  Variable Phi : state. 
+
+  Reserved Notation "x == y" (at level 70, no associativity). 
+  Reserved Notation "x ==e y" (at level 70, no associativity). 
+  
+  Section inner_equiv. 
+  Variable R : forall t, U t -> V t -> Prop. 
+  Notation "x -- y" := (R _ x y) (at level 70, no associativity). 
+    
+  Inductive expr_equiv : forall t,  expr Phi U t -> expr Phi V t -> Prop :=
+  | Eq_read : forall t v, Eread Phi U t v == Eread Phi V t v
+  | Eq_read_rf : forall n t v adr1 adr2, 
+                   adr1 -- adr2 -> 
+                   Eread_rf Phi U n t v adr1 == Eread_rf Phi V n t v adr2
+  | Eq_builtin : forall args res (f : builtin args res) dl1 dl2, 
+                   Common.DList.pointwise R args dl1 dl2 ->
+                   Ebuiltin Phi U args res f dl1 == Ebuiltin Phi V args res f dl2
+  | Eq_constant : forall ty c, Econstant Phi U ty c == Econstant Phi V ty c
+  | Eq_mux : forall t c1 c2 l1 l2 r1 r2, 
+               c1 -- c2 -> l1 -- l2 -> r1 -- r2 -> 
+               Emux Phi U t c1 l1 r1 ==  Emux Phi V t c2 l2 r2
+                    
+  | Eq_fst : forall (l : list type) (t : type) dl1 dl2, 
+               dl1 -- dl2 -> 
+               Efst Phi U l t dl1 == Efst Phi V l t dl2
+
+  | Eq_snd : forall (l : list type) (t : type) dl1 dl2, 
+               dl1 -- dl2 -> 
+               Esnd Phi U l t dl1 == Esnd Phi V l t dl2
+
+  | Eq_nth : forall (l : list type) (t : type) (v : Common.var l t)  dl1 dl2, 
+               dl1 -- dl2 -> 
+               Enth Phi U l t v dl1 == Enth Phi V l t v dl2
+
+  | Eq_tuple : forall (l : list type) dl1 dl2, 
+                 Common.DList.pointwise R l dl1 dl2 ->
+               Etuple Phi U l dl1 == Etuple Phi V l dl2
+                            where "x == y" := (expr_equiv _ x y). 
+  
+  Inductive effect_equiv : forall t,  option (effect U t) -> option (effect V t) -> Prop :=
+  | Eq_none : forall t, effect_equiv t None None
+  | Eq_write : forall t v1 v2 we1 we2, 
+                 v1 -- v2 -> we1 -- we2 -> 
+                 Some (effect_reg_write U t v1 we1) ==e Some  (effect_reg_write V t v2 we2)
+  | Eq_write_rf : forall n t v1 v2 adr1 adr2 we1 we2, 
+                    v1 -- v2 -> adr1 -- adr2 -> we1 -- we2 -> 
+                    Some (effect_regfile_write U n t v1 adr1 we1) ==e 
+                         Some (effect_regfile_write V n t v2 adr2 we2)
+                                  where "x ==e y" := (effect_equiv _ x y). 
+ 
+  Definition effects_equiv : effects Phi U -> effects Phi V -> Prop := 
+    Common.Tuple.pointwise _ _ effect_equiv Phi. 
+    
+  End inner_equiv. 
+ 
+  Inductive Gamma : Type :=
+  | nil : Gamma
+  | cons : forall t, U t -> V t -> Gamma -> Gamma. 
+  
+  Inductive In t (x : U t) (y : V t) : Gamma -> Prop :=
+  | In_ok : forall Gamma x' y', x' = x -> y' = y ->
+              In t x y (cons t x' y' Gamma )
+  | In_skip : forall Gamma x' y', 
+                In t x y Gamma -> 
+                In t x y (cons t x' y' Gamma ). 
+
+  Definition R G := fun t x y => In t x y G.  
+
+  Reserved Notation "G |- x ==b y" (at level 70, no associativity). 
+  Notation "G |- x -- y" := (In _ x y G) (at level 70, no associativity). 
+
+  Inductive block_equiv t : forall (G : Gamma), block Phi U t -> block Phi V t -> Prop :=
+  | Eq_end : forall G (v1 : U t) v2 g1 g2 e1 e2, 
+               G |- v1 -- v2 -> G |- g1 -- g2 -> effects_equiv (R G) e1 e2 ->
+               G |- telescope_end Phi U _ (v1, g1, e1) ==b telescope_end Phi V _ (v2,g2, e2 ) 
+  | Eq_bind : forall G a (e1 : expr Phi U a) e2 (k1 : U a -> block Phi U t) k2,
+                expr_equiv (R G) _ e1 e2 -> 
+                (forall v1 v2, G |- v1 -- v2 -> cons _ v1 v2 G |- k1 v1 ==b k2 v2) ->
+                G |- telescope_bind Phi U _ a e1 k1 ==b telescope_bind Phi V _ a e2 k2                
+                 where "G |- x ==b y" := (block_equiv _ G x y). 
+End equiv. 
